Implementations of Agile.DH using P256

code/hpke/Hacl.Impl.Generic.DH.fst
@@ -2,6 +2,7 @@ module Hacl.Impl.Generic.DH
 
 open FStar.HyperStack
 open FStar.HyperStack.All
+module HST = FStar.HyperStack.ST
 
 open Lib.Buffer
 open Lib.IntTypes
@@ -32,12 +33,15 @@ let dh_st (a:DH.algorithm) =
   -> ST UInt32.t
      (requires fun h0 ->
        (a = DH.DH_Curve25519 ==> Vale.X64.CPU_Features_s.(adx_enabled /\ bmi2_enabled)) /\
+       (a = DH.DH_P256 ==> Lib.ByteSequence.(
+           nat_from_bytes_le (as_seq h0 k) >= 1 /\
+           nat_from_bytes_le (as_seq h0 k) < Spec.ECDSAP256.Definition.prime_p256_order)) /\
        live h0 o /\ live h0 k /\ live h0 i /\
        disjoint o i /\ disjoint o k)
      (ensures fun h0 result h1 -> modifies (loc o) h0 h1 /\ (
        let output = DH.dh a (as_seq h0 k) (as_seq h0 i) in
        match result with
-       | 0ul -> Some? output /\ as_seq h1 o == Some?.v output // DH succeeded
+       | 0ul -> Some? output /\ as_seq h1 o `Seq.equal` Some?.v output // DH succeeded
        | 1ul -> None? output
        | _ -> False))
 
@@ -48,11 +52,14 @@ let secret_to_public_st (a: DH.algorithm) =
   -> Stack UInt32.t
     (requires fun h0 ->
       (a = DH.DH_Curve25519 ==> Vale.X64.CPU_Features_s.(adx_enabled /\ bmi2_enabled)) /\
+      (a = DH.DH_P256 ==> Lib.ByteSequence.(
+           nat_from_bytes_le (as_seq h0 i) >= 1 /\
+           nat_from_bytes_le (as_seq h0 i) < Spec.ECDSAP256.Definition.prime_p256_order)) /\
       live h0 o /\ live h0 i /\ disjoint o i)
     (ensures  fun h0 result h1 -> modifies (loc o) h0 h1 /\
       (let output = DH.secret_to_public a (as_seq h0 i) in
       match result with
-      | 0ul -> Some? output /\ as_seq h1 o == Some?.v output
+      | 0ul -> Some? output /\ as_seq h1 o `Seq.equal` Some?.v output
       | 1ul -> None? output
       | _ -> False))
 
@@ -90,3 +97,42 @@ let dh_c64 : dh_st (DH.DH_Curve25519) = fun o k i ->
   let res = if lbytes_eq o zeros then 1ul else 0ul in
   pop_frame();
   res
+
+// TODO: After unification of error codes, this should be removed
+inline_for_extraction noextract
+let change_error_code (r:uint64) : Pure UInt32.t
+  (requires v r = 0 \/ v r = pow2 64 - 1)
+  (ensures fun r' -> UInt32.v r' <= 1 /\ (UInt32.v r' = 0 <==> v r = 0))
+  = let r' = logand r (u64 1) in
+    logand_mask r (u64 1) 1;
+    let r' = cast U32 SEC r' in
+    Lib.RawIntTypes.u32_to_UInt32 r'
+
+inline_for_extraction noextract
+let secret_to_public_p256 : secret_to_public_st (DH.DH_P256) = fun o i ->
+  let res = Hacl.Impl.P256.DH.ecp256dh_i o i in
+  change_error_code res
+
+let rec nat_from_bytes_le_zero_is_zero (n:size_nat{n >= 1}) (s:Lib.ByteSequence.lbytes n)
+  : Lemma (requires s `Seq.equal` Lib.Sequence.create n (u8 0))
+          (ensures Lib.ByteSequence.nat_from_bytes_le s == 0)
+  = let open Lib.Sequence in
+    let open Lib.ByteSequence in
+    if n = 1 then nat_from_intseq_le_lemma0 s
+    else (
+      nat_from_intseq_le_slice_lemma s 1;
+      nat_from_bytes_le_zero_is_zero (n-1) (slice s 1 n);
+      nat_from_intseq_le_lemma0 (slice s 0 1)
+   )
+
+inline_for_extraction noextract
+let dh_p256 : dh_st (DH.DH_P256) = fun o k i ->
+  push_frame();
+  let tmp = create (size 64) (u8 0) in
+  (**) let h0 = HyperStack.ST.get() in
+  (**) nat_from_bytes_le_zero_is_zero 32 (as_seq h0 (gsub tmp (size 0) (size 32)));
+  (**) nat_from_bytes_le_zero_is_zero 32 (as_seq h0 (gsub tmp (size 32) (size 32)));
+  let res = Hacl.Impl.P256.DH.ecp256dh_r tmp i k in
+  copy o tmp;
+  pop_frame();
+  change_error_code res
